yui

HeadReduction.v
@@ -7,239 +7,306 @@ Require Import ssreflect LAF Semantics NormalisationTheory Basic.
 
 Section HeadReduction.
 
-Context (LAF:LAFs).
+  Context (LAF:LAFs).
 
-Definition WDep A := {w: World LAF & A w}.
+  Definition WDep A := {w: World LAF & A w}.
 
-Record AbstractMachines :=
-  {
-    ETerms : Type;
-    ESoContexts: LAF.(QWorld) -> Type;
-    EPos   : Type;
-    ENeg   : Type;
-    Closures: World LAF -> Type;
-    EContext: Contexts wextends EPos (ENeg + WDep Closures) ETerms ESoContexts;
-    clNeg w : (@Neg LAF w * EContext w) -> Closures w;
-    clNegInj : forall w cl1 cl2, @clNeg w cl1 = @clNeg w cl2 -> cl1 = cl2;
-    EvalTerms {qLab} : ESoContexts qLab -> Terms qLab -> ETerms
-  }
-.
+  Record AbstractMachines :=
+    {
+      ETerms : Type;
+      ESoContexts: LAF.(QWorld) -> Type;
+      EPos   : Type;
+      ENeg   : Type;
+      Closures: World LAF -> Type;
+      EContext: Contexts wextends EPos (ENeg + WDep Closures) ETerms ESoContexts;
+      clNeg w : (Neg w * EContext w) -> Closures w;
+      clNegInj : forall w cl1 cl2, @clNeg w cl1 = @clNeg w cl2 -> cl1 = cl2;
+      EvalTerms {qLab} : ESoContexts qLab -> Terms qLab -> ETerms
+    }
+  .
 
-Variable AM: AbstractMachines.
+  Notation "<< x , y >>" := (inr {{ _ , (clNeg (x,y)) }} ).
+  Notation "<< x | y >>" := (existS (fun w => Command w * EContext _ w) _ (x,y)).
 
-Definition VNeg := sum AM.(ENeg) (WDep AM.(Closures)).
-Notation "<< x , y >>" := (inr {{ _ , (clNeg (x,y)) }} ).
+  Section AbstractMachines.
 
-Definition ECommand := WDep (fun w => @Command LAF w * EContext AM w).
-Notation "<< x | y >>" := (existS (fun w => @Command LAF w * EContext _ w) _ (x,y)).
+    Variable AM: AbstractMachines.
 
-Definition EDec := @Dec AM.(ETerms) AM.(EPos) VNeg.
+    Definition VNeg := sum AM.(ENeg) (WDep AM.(Closures)).
 
-Lemma EvalDec : 
-  forall w (rho:AM.(EContext) w) st, @TermDec LAF w st ->  @EDec st.
-Proof.
-  move => w rho.
-  elim => [v | v | v | s1 H1 s2 H2 v | s H v]; inversion v =>//=.
-  exact (leafP (rho.(readp) X)).
-  exact (leafN(<< X , rho >>)).
-  exact dummy.
-  exact (node (H1 X)(H2 X0)).
-  exact (qnode (EvalTerms (readE rho) X) (H X0)).
-Defined.
-Unset Implicit Arguments.
+    Definition ECommand := WDep (fun w => Command w * EContext AM w).
 
-Definition ETriple := VNeg * {p:Patterns LAF & EDec (LAF.(@PatDec) p)}.
+    Definition EDec := @Dec AM.(ETerms) AM.(EPos) VNeg.
 
-Set Implicit Arguments.
-Unset Strict Implicit.
-Set Maximal Implicit Insertion.
+    Lemma EvalDec : 
+      forall w (rho:AM.(EContext) w) st, TermDec w st ->  EDec st.
+    Proof.
+      move => w rho.
+      elim => [v | v | v | s1 H1 s2 H2 v | s H v]; inversion v =>//=.
+      exact (leafP (rho.(readp) X)).
+      exact (leafN(<< X , rho >>)).
+      exact dummy.
+      exact (node (H1 X)(H2 X0)).
+      exact (qnode (EvalTerms (readE rho) X) (H X0)).
+    Defined.
+    Unset Implicit Arguments.
 
-Notation "<< x | y | z >>" := (x, {{ y,z }}).
+    Definition ETriple := VNeg * {p:Patterns LAF & EDec (PatDec p)}.
 
-Inductive ECom2ETri : ECommand ->  ETriple -> Prop :=
-| head1:
-    forall w (xn:w.(NLab)) p d rho,
-    ECom2ETri << select xn (pos p d) | rho >> << readn rho xn | p | EvalDec rho d >>
-| head2:
-    forall w (tn:@Neg LAF w) p d rho,
-    ECom2ETri << cut tn (pos p d) | rho >> <<<< tn,rho >>| p | EvalDec rho d >>
-.
+    Set Implicit Arguments.
+    Unset Strict Implicit.
+    Set Maximal Implicit Insertion.
 
-Inductive ETri2ECom : ETriple ->  ECommand -> Prop :=
-| head3:
-    forall w (f:Reifiable w) p d rho c,
-      f p =cis= c
-      -> ETri2ECom <<<< rei f,rho >> | p | d >> << c | extends d rho >>
-.
+    Notation "<< x | y | z >>" := (x, {{ y,z }}).
 
-Lemma ETri2EComRed : forall w (f:Reifiable w) p d rho x,
-                       ETri2ECom <<<< rei f,rho >> | p | d >> x
-                        -> forall c, f p =cis= c
+    Inductive ECom2ETri : ECommand ->  ETriple -> Prop :=
+    | head1:
+        forall w (xn:w.(NLab)) p d rho,
+          ECom2ETri << select xn (pos p d) | rho >> << readn rho xn | p | EvalDec rho d >>
+    | head2:
+        forall w (tn:Neg w) p d rho,
+          ECom2ETri << cut tn (pos p d) | rho >> <<<< tn,rho >>| p | EvalDec rho d >>
+    .
+
+    Inductive ETri2ECom : ETriple ->  ECommand -> Prop :=
+    | head3:
+        forall w (f:Reifiable w) p d rho c,
+          f p =cis= c
+          -> ETri2ECom <<<< rei f,rho >> | p | d >> << c | extends d rho >>
+    .
+
+    Lemma ETri2EComRed : forall w (f:Reifiable w) p d rho x,
+                           ETri2ECom <<<< rei f,rho >> | p | d >> x
+                           -> forall c, f p =cis= c
                                -> x = << c | extends d rho >>.
-Proof.
-  move => w f p d rho x H.
-  have: (forall f' rho', 
-           clNeg(rei f,rho) = clNeg (rei f',rho')
-           -> forall c' : Command _ (LAF:=LAF),
-               f' p =cis= c' ->
-               x =
-               {{wextends (l:=LAF) (PatDec (l:=LAF) p) w,
-                 (c', extends (c:=EContext AM) (w:=w) d rho')}}).
-  refine
-    (match H as J in ETri2ECom K K' 
-           return 
-           (match K with
-              | (inr {{ _ , closure }}, {{ p', d'}})
-                => forall f' rho', 
-                    closure = clNeg (rei f',rho')
-                    -> forall c', 
-                        f' p' =cis= c'
-                        -> K' =<< c' | extends d' rho' >>
-              | _ => True 
-            end : Prop) with
-       | head3 _ _ _ _ _ _ _ => _
-     end)
-  .
-  move => f' rho' H0 c' H1.
-  move:(clNegInj H0); clear H0 H; move => [H H0].
-  rewrite H0;clear H0.
-  inversion c0; clear c0.
-  rewrite H in H2;clear H.
-  inversion H1; clear H1.
-  rewrite <- H2 in H3; clear H2.
-  inversion H3; clear H3.
-  rewrite H0 in H1; clear H0.
-  rewrite H4 in H1; clear H4.
-  rewrite H1.
-  done.
-  apply.
-  done.
-Qed.
+    Proof.
+      move => w f p d rho x H.
+      have: (forall f' rho', 
+               clNeg(rei f,rho) = clNeg (rei f',rho')
+               -> forall c' : Command _ (LAF:=LAF),
+                   f' p =cis= c' ->
+                   x =
+                   {{ wextends (l:=LAF) (PatDec (l:=LAF) p) w,
+                     (c', extends (c:=EContext AM) (w:=w) d rho')}}).
+      refine
+        (match H as J in ETri2ECom K K' 
+               return 
+               (match K with
+                  | (inr {{ _ , closure }}, {{ p', d'}})
+                    => forall f' rho', 
+                        closure = clNeg (rei f',rho')
+                        -> forall c', 
+                            f' p' =cis= c'
+                            -> K' =<< c' | extends d' rho' >>
+                  | _ => True 
+                end : Prop) with
+           | head3 _ _ _ _ _ _ _ => _
+         end)
+      .
+      move => f' rho' H0 c' H1.
+      move:(clNegInj H0); clear H0 H; move => [H H0].
+      rewrite H0;clear H0.
+      inversion c0; clear c0.
+      rewrite H in H2;clear H.
+      inversion H1; clear H1.
+      rewrite <- H2 in H3; clear H2.
+      inversion H3; clear H3.
+      rewrite H0 in H1; clear H0.
+      rewrite H4 in H1; clear H4.
+      rewrite H1.
+      done.
+      apply.
+      done.
+    Qed.
 
-Inductive HeadReduction : ETriple ->  ETriple -> Prop :=
-| head123 a b c : ETri2ECom a b -> ECom2ETri b c -> HeadReduction a c.
+    Inductive HeadReduction : ETriple ->  ETriple -> Prop :=
+    | head123 a b c : ETri2ECom a b -> ECom2ETri b c -> HeadReduction a c.
 
-Section Normalisation.
+    Section Normalisation.
 
-  Definition HeadStruct := 
-    {|
-      STerms   := ETerms AM;
-      Valuations := ESoContexts AM;
-      SLab     := EPos AM;
-      SPos     := { p:Patterns LAF & EDec (PatDec p)};
-      SNeg     := VNeg;
-      orth     := SN HeadReduction ;
-      SContexts := EContext AM;
-      tild p v := {{ p, v }};
-      SemTerms := @EvalTerms AM;
-      I w rho f := << rei f, rho >>
-    |}
-  .
+      Definition HeadStruct := 
+        {|
+          STerms   := ETerms AM;
+          Valuations := ESoContexts AM;
+          SLab     := EPos AM;
+          SPos     := { p:Patterns LAF & EDec (PatDec p)};
+          SNeg     := VNeg;
+          orth     := SN HeadReduction ;
+          SContexts := EContext AM;
+          tild p v := {{ p, v }};
+          SemTerms := @EvalTerms AM;
+          I w rho f := << rei f, rho >>
+        |}
+      .
 
-  Variable WF: well_founded (relation (LAF:=LAF)).
+      Variable WF: well_founded (relation (LAF:=LAF)).
 
-  Definition HeadRAlg :=
-    {|
-      modelStructure := HeadStruct;
-      welf := WF;
-      SemSorts s r := True;
-      SemSoCont w Sigma sigma := True;
-      SemSoCompat qLab Sigma r s sigma := fun _ _ => Logic.I;
-      SemAtom a tl vp := True;
-      SemAtom_eq qLab sigma a b tl := fun _ _ => Logic.I
-    |}.
+      Definition HeadRAlg :=
+        {|
+          modelStructure := HeadStruct;
+          welf := WF;
+          SemSorts s r := True;
+          SemSoCont w Sigma sigma := True;
+          SemSoCompat qLab Sigma r s sigma := fun _ _ => Logic.I;
+          SemAtom a tl vp := True;
+          SemAtom_eq qLab sigma a b tl := fun _ _ => Logic.I
+        |}.
 
-  Lemma SemEvalDec {w} : forall rho st (v:@TermDec LAF w st), 
-                        SemDec (M:= HeadStruct) rho v = EvalDec rho v.
-  Proof.
-    move => rho.
-    elim => [v | v | v | s1 H1 s2 H2 v | s H v]; dependent inversion v =>//=.
-      by elim n.
-      by rewrite H1 H2.
-      by rewrite H.
-  Qed.
+      Lemma SemEvalDec {w} : forall rho st (v:TermDec w st), 
+                               SemDec (M:= HeadStruct) rho v = EvalDec rho v.
+      Proof.
+        move => rho.
+        elim => [v | v | v | s1 H1 s2 H2 v | s H v]; dependent inversion v =>//=.
+                                                    by elim n.
+          by rewrite H1 H2.
+            by rewrite H.
+      Qed.
 
-  Lemma Rem61 : forall w (c:@Command LAF w) rho, ECom2ETri << c | rho >> (SemC (M:= HeadStruct) rho c).
-  Proof.
-    move => w [[f] | xn]; move => [p v] rho /=; rewrite SemEvalDec.
-    apply: head2.
-    apply: head1.
-  Qed.
+      Lemma Rem61 : forall w (c:Command w) rho, ECom2ETri << c | rho >> (SemC (M:= HeadStruct) rho c).
+      Proof.
+        move => w [[f] | xn]; move => [p v] rho /=; rewrite SemEvalDec.
+        apply: head2.
+        apply: head1.
+      Qed.
 
-  Lemma Rem61' : forall w (c:@Command LAF w) rho x, 
-                   ECom2ETri << c | rho >> x
-                                    -> x = (SemC (M:= HeadStruct) rho c).
-  Proof.
-    move => w [[f] | xn]; move => [p v] rho x /=; rewrite SemEvalDec => H.
-    refine
-      (match H as J in ECom2ETri K K' 
-             return 
-             (match K with
-               | {{ w', (cut tn' (pos p' v'), rho') }} 
-                 => K' = << << tn', rho' >> | p' | EvalDec rho' v' >>
-               | {{ w', (_, rho') }} => True 
-              end : Prop) with
-         | head1 _ _ _ _ _ => Logic.I
-         | head2 _ _ _ _ _ => eq_refl
-       end)
-    .
-    refine (match H as J in ECom2ETri K K' 
-             return 
-             (match K with
-               | {{ w', (select xn' (pos p' v'), rho') }} 
-                 => K' = << readn (c:=EContext AM) (w:=w') rho' xn' | p' | EvalDec rho' v' >>
-               | {{ w', (_, rho') }} => True 
-              end : Prop) with
-         | head1 _ _ _ _ _ => eq_refl
-         | head2 _ _ _ _ _ => Logic.I
-       end)
-    .
-  Qed.
+      Lemma Rem61' : forall w (c:Command w) rho x, 
+                       ECom2ETri << c | rho >> x
+                                        -> x = (SemC (M:= HeadStruct) rho c).
+      Proof.
+        move => w [[f] | xn]; move => [p v] rho x /=; rewrite SemEvalDec => H.
+        refine
+          (match H as J in ECom2ETri K K' 
+                 return 
+                 (match K with
+                    | {{ w', (cut tn' (pos p' v'), rho') }} 
+                      => K' = << << tn', rho' >> | p' | EvalDec rho' v' >>
+                    | {{ w', (_, rho') }} => True 
+                  end : Prop) with
+             | head1 _ _ _ _ _ => Logic.I
+             | head2 _ _ _ _ _ => eq_refl
+           end)
+        .
+        refine (match H as J in ECom2ETri K K' 
+                      return 
+                      (match K with
+                         | {{ w', (select xn' (pos p' v'), rho') }} 
+                           => K' = << readn (c:=EContext AM) (w:=w') rho' xn' | p' | EvalDec rho' v' >>
+                         | {{ w', (_, rho') }} => True 
+                       end : Prop) with
+                  | head1 _ _ _ _ _ => eq_refl
+                  | head2 _ _ _ _ _ => Logic.I
+                end)
+        .
+      Qed.
 
 
 
-  Lemma StabHN w :
+      Lemma StabHN w :
         forall (f: Reifiable w) (rho: HeadRAlg.(SContexts) w) (p: Patterns LAF)
           l Delta (tl:STList HeadRAlg l) (v: SDec (PatDec p)) c,
           f p =cis= c
           -> SemTDec Delta tl v
           -> orth (SemC (extends v rho) c)
           -> orth (I rho f, tild p v).
-  Proof.
-    move => /= f rho p l Delta tl v c H0 _ H2.
-    apply toSN => x' H3.
-    inversion H3.
-    clear a c0 H3 H4 H5.
-    move: (ETri2EComRed H H0).
-    clear H => H.
-    rewrite H in H1; clear H H0 b.
-    case: c H1 H2 => [[f'] | xn] ; move => [p' v'] /= ; rewrite SemEvalDec => H1 H2;
-      move: (Rem61' H1); clear H1 => H1;
-      rewrite H1 => /=; rewrite SemEvalDec => //.
-  Qed.
+      Proof.
+        move => /= f rho p l Delta tl v c H0 _ H2.
+        apply toSN => x' H3.
+        inversion H3.
+        clear a c0 H3 H4 H5.
+        move: (ETri2EComRed H H0).
+        clear H => H.
+        rewrite H in H1; clear H H0 b.
+        case: c H1 H2 => [[f'] | xn] ; move => [p' v'] /= ; rewrite SemEvalDec => H1 H2;
+          move: (Rem61' H1); clear H1 => H1;
+          rewrite H1 => /=; rewrite SemEvalDec => //.
+      Qed.
 
-  Variable TC: forall w st (rho:HeadRAlg.(SContexts) w) Gamma l (Delta:TypingDec st l) tl v, 
-                 SemCont Gamma rho
-                 -> SemTDec Delta (SemTermList (readE rho) tl) v
-                 -> SemCont (Textends [Delta,tl] Gamma) (extends v rho).
-  
-  Definition HeadModel := 
-    {|
-      M0 := HeadRAlg;
-      TypingCorr := @TC;
-      Stability  := @StabHN
-    |}.
+      Variable TC: forall w st (rho:HeadRAlg.(SContexts) w) Gamma l (Delta:TypingDec st l) tl v, 
+                     SemCont Gamma rho
+                     -> SemTDec Delta (SemTermList (readE rho) tl) v
+                     -> SemCont (Textends [Delta,tl] Gamma) (extends v rho).
+      
+      Definition HeadModel := 
+        {|
+          M0 := HeadRAlg;
+          TypingCorr := @TC;
+          Stability  := @StabHN
+        |}.
 
-  Theorem HeadNormalisation: 
-    forall w Gamma c (rho: HeadModel.(SContexts) w),
-      CommandTyping Gamma c -> SemCont Gamma rho -> SN HeadReduction (SemC rho c).
-  Proof.
-    move => w Gamma c rho H H1.
-    elim: (adequacy HeadModel Gamma) => [_ [_ [_ [_ H']]]]. 
-    by move:(H' c H rho H1).
-  Qed.
+      Theorem HeadNormalisation: 
+        forall w Gamma c (rho: HeadModel.(SContexts) w),
+          CommandTyping Gamma c -> SemCont Gamma rho -> SN HeadReduction (SemC rho c).
+      Proof.
+        move => w Gamma c rho H H1.
+        elim: (adequacy HeadModel Gamma) => [_ [_ [_ [_ H']]]]. 
+          by move:(H' c H rho H1).
+      Qed.
 
-End Normalisation.
+    End Normalisation.
+  End AbstractMachines.
+
+  Section SyntacticMachines.
+
+    Definition asAbstractMachine (w0 : World LAF)
+               ClosuresV EContextV clNegV clNegInjV EvalTermsV :=
+      {|
+        ETerms    := Terms w0.(QLab);
+        ESoContexts := SoContexts;
+        EPos      := PLab w0;
+        ENeg      := NLab w0;
+        Closures  := ClosuresV;
+        EContext  := EContextV;
+        clNeg     := clNegV;
+        clNegInj  := clNegInjV;
+        EvalTerms := EvalTermsV
+      |}
+    .
+
+    Class SyntacticMachines {ClosuresV EContextV clNegV clNegInjV EvalTermsV}
+      := {
+          asAM w: SClass (@asAbstractMachine w (ClosuresV w) (EContextV w) 
+                                             (clNegV w) (clNegInjV w) (EvalTermsV w));
+          ident w: (EContextV w).(Csupport) w;
+          identP w: forall xp:w.(PLab), readp (ident w) xp = xp;
+          identN w: forall xn:w.(NLab), readn (ident w) xn = inl xn
+        }.
+
+    Context `(SM:SyntacticMachines). 
+
+    Variable WF: well_founded (relation (LAF:=LAF)).
+
+    Variable TC: forall w0 w st (rho:(HeadRAlg (get (asAM w0)) WF).(SContexts) w) Gamma l (Delta:TypingDec st l) tl v, 
+                   SemCont Gamma rho
+                   -> SemTDec Delta (SemTermList (readE rho) tl) v
+                   -> SemCont (Textends [Delta,tl] Gamma) (extends v rho).
+
+    Theorem SHeadNormalisation:
+        forall w Gamma (c : Command w), 
+          CommandTyping Gamma c
+          -> SN HeadReduction (SemC (M := HeadStruct (get (asAM w)))
+                                   (ident w)
+                                   c).
+    Proof.
+      move => w Gamma c H.      
+      apply (HeadNormalisation (AM := get (asAM w))
+                               (Gamma := Gamma)
+                               (TC := @TC w)
+            ) => //.
+      rewrite /SemCont.
+      simpl.
+      split => //.
+      split => [xp | xn] //.
+      rewrite /Pard/getA/getTerms/ex2/ex1.
+      elim (Treadn (t:=TContext) (w:=w) Gamma xn) => l [M tl].
+      rewrite identN /SemNeg/ortho.
+      elim => p v H0.
+      simpl.
+      apply toSN => x' H3.
+      inversion H3.
+      inversion H1.
+    Qed.
+
+  End SyntacticMachines.
 
 End HeadReduction.
 
